# Retrieved on 14 Jan 2022
# Source: https://cso.kmi.open.ac.uk/schema/cso
# See also: https://cso.kmi.open.ac.uk/about
# Authors: Salatino, Angelo A., Thiviyan Thanapalasingam, Andrea Mannocci, Francesco Osborne, and Enrico Motta
# License: Creative Commons Attribution 4.0

@prefix : <http://cso.kmi.open.ac.uk/schema/cso#> .
@prefix owl: <http://www.w3.org/2002/07/owl#> .
@prefix rdf: <http://www.w3.org/1999/02/22-rdf-syntax-ns#> .
@prefix xml: <http://www.w3.org/XML/1998/namespace> .
@prefix xsd: <http://www.w3.org/2001/XMLSchema#> .
@prefix rdfs: <http://www.w3.org/2000/01/rdf-schema#> .
@prefix skos: <http://www.w3.org/2004/02/skos/core#> .
@base <http://cso.kmi.open.ac.uk/schema/cso#> .

<http://cso.kmi.open.ac.uk/schema/cso#> rdf:type owl:Ontology ;
                                         owl:imports <https://www.w3.org/2009/08/skos-reference/skos.rdf> .

#################################################################
#    Object Properties
#################################################################

###  http://cso.kmi.open.ac.uk/schema/cso#contributesTo
:contributesTo rdf:type owl:ObjectProperty ;
               rdfs:domain :Topic ;
               rdfs:range :Topic ;
               rdfs:comment "We use this relation to indicate that the research output of one topic contributes to another." ;
               rdfs:label "contributes to"@en .


###  http://cso.kmi.open.ac.uk/schema/cso#preferentialEquivalent
:preferentialEquivalent rdf:type owl:ObjectProperty ;
                        rdfs:subPropertyOf :relatedEquivalent ,
                                           skos:related ;
                        rdf:type owl:FunctionalProperty ;
                        rdfs:domain :Topic ;
                        rdfs:range :Topic ;
                        rdfs:comment "We use this relationship to declare that the subject topic need to use the label of the object topic for presentation purposes." ;
                        rdfs:label "preferential equivalent"@en .


###  http://cso.kmi.open.ac.uk/schema/cso#relatedEquivalent
:relatedEquivalent rdf:type owl:ObjectProperty ;
                   rdfs:subPropertyOf skos:related ;
                   rdf:type owl:SymmetricProperty ,
                            owl:TransitiveProperty ;
                   rdfs:domain :Topic ;
                   rdfs:range :Topic ;
                   rdfs:comment "We use this relationship to identify that two potentially distinct research concepts are treated as equivalent in the context of the CSO." ;
                   rdfs:label "related equivalent"@en ;
                   skos:note "Different from skos:exactMatch" .


###  http://cso.kmi.open.ac.uk/schema/cso#subTopicOf
:subTopicOf rdf:type owl:ObjectProperty ;
            owl:inverseOf :superTopicOf ;
            rdf:type owl:TransitiveProperty ;
            rdfs:domain :Topic ;
            rdfs:range :Topic ;
            rdfs:comment "We use this relation to indicate that a :Topic is a sub-area of another one. This is the inverse of :superTopicOf" ;
            rdfs:label "sub-topic of"@en .


###  http://cso.kmi.open.ac.uk/schema/cso#superTopicOf
:superTopicOf rdf:type owl:ObjectProperty ;
              rdfs:subPropertyOf skos:narrower ;
              rdf:type owl:TransitiveProperty ;
              rdfs:domain :Topic ;
              rdfs:range :Topic ;
              rdfs:comment "We use this relation to indicate that a :Topic is a super-area of another one." ;
              rdfs:label "super-topic of"@en .


#################################################################
#    Classes
#################################################################

###  http://cso.kmi.open.ac.uk/schema/cso#Topic
:Topic rdf:type owl:Class ;
       rdfs:subClassOf skos:Concept .
